---
title: "2. Logical Equivalence, Normal Forms (DNF, CNF, ANF)"
author: "Zakhar Podyakov"
date: "September 16, 2025"
format: html
---

#### 1. Summary

##### 1.1 Classification of Logical Formulas
In logic, any declarative statement, or **proposition**, can be classified based on its truth values across all possible scenarios.

*   A **Tautology** is a formula that is *always true*, regardless of the truth values of its variables. For example, the formula $p \lor \neg p$ is a tautology because it is true whether $p$ is true or false.
*   A **Contradiction** is a formula that is *always false*. The formula $p \land \neg p$ is a contradiction.
*   A **Contingency** is a formula that is neither a tautology nor a contradiction. Its truth value *depends* on the truth values of its variables. For example, $p \land q$ is a contingency.

A formula is considered **satisfiable** if there exists at least one assignment of truth values to its variables that makes the entire formula true. Both tautologies and contingencies are satisfiable, while contradictions are not.

##### 1.2 Logical Equivalence
Two propositions, $P_1$ and $P_2$, are **logically equivalent** if they have the exact same truth table. This means that for every possible combination of truth values for their variables, $P_1$ and $P_2$ will have the same resulting truth value. We denote this equivalence using the symbol $\equiv$. For example, the implication $a \rightarrow b$ is logically equivalent to $\neg a \lor b$, written as $a \rightarrow b \equiv \neg a \lor b$.

Proving logical equivalence can be done by constructing a truth table for both expressions or by using a series of known equivalences (laws) to transform one expression into the other.

##### 1.3 Key Logical Equivalences (Laws)

*   **Identity Laws:** $p \lor F \equiv p$, $p \land T \equiv p$
*   **Domination Laws:** $p \lor T \equiv T$, $p \land F \equiv F$
*   **Idempotent Laws:** $p \lor p \equiv p$, $p \land p \equiv p$
*   **Double Negation Law:** $\neg(\neg p) \equiv p$
*   **Commutative Laws:** $p \lor q \equiv q \lor p$, $p \land q \equiv q \land p$
*   **Associative Laws:** $(p \lor q) \lor r \equiv p \lor (q \lor r)$, $(p \land q) \land r \equiv p \land (q \land r)$
*   **Distributive Laws:** $p \lor (q \land r) \equiv (p \lor q) \land (p \lor r)$, $p \land (q \lor r) \equiv (p \land q) \lor (p \land r)$
*   **De Morgan's Laws:** These are crucial for simplifying negated expressions: $\neg(p \land q) \equiv \neg p \lor \neg q$ and $\neg(p \lor q) \equiv \neg p \land \neg q$. *Correction from source material: The slides correctly apply the laws, but it's important to state explicitly that the operator between the terms is also inverted (AND to OR, OR to AND).*
*   **Absorption Laws:** $p \lor (p \land q) \equiv p$, $p \land (p \lor q) \equiv p$
*   **Implication Equivalence:** $p \rightarrow q \equiv \neg p \lor q$
*   **Bi-implication Equivalence:** $p \leftrightarrow q \equiv (p \rightarrow q) \land (q \rightarrow p) \equiv (p \land q) \lor (\neg p \land \neg q)$

##### 1.4 Normal Forms: DNF and CNF
A logical formula can be standardized into a **normal form**.

*   **Disjunctive Normal Form (DNF):** A formula is in DNF if it is a *disjunction (ORs) of conjunctions (ANDs)* of literals (a variable or its negation). A DNF expression can be derived from a truth table by taking every row where the formula is true and creating an AND clause that matches that row's inputs. All these AND clauses are then ORed together. This is often called a "sum of products."
*   **Conjunctive Normal Form (CNF):** A formula is in CNF if it is a *conjunction (ANDs) of disjunctions (ORs)* of literals. A CNF expression can be derived from a truth table by taking every row where the formula is false, creating an OR clause from the *negation* of that row's inputs, and then ANDing all these OR clauses together. This is often called a "product of sums."

##### 1.5 Algebraic Normal Form (ANF)
**Algebraic Normal Form (ANF)**, also known as a **Zhegalkin polynomial**, re-expresses a logical formula as a polynomial modulo 2. In this system, multiplication corresponds to the logical AND ($\land$), and addition corresponds to the logical XOR ($\oplus$).

The key translations are:
*   $p \land q \equiv p \cdot q$ (or simply $pq$)
*   $p \oplus q$ (XOR)
*   $\neg p \equiv p \oplus 1$
*   $p \lor q \equiv p \oplus q \oplus pq$
*   $p \rightarrow q \equiv 1 \oplus p \oplus pq$
*   $p \leftrightarrow q \equiv 1 \oplus p \oplus q$

Any boolean expression can be uniquely converted into this polynomial form, which is useful in cryptography and circuit design.

---

#### 2. Definitions

*   **Proposition**: A declarative statement that is either true or false.
*   **Tautology**: A logical formula that is true for all possible truth value assignments to its variables.
*   **Contradiction**: A logical formula that is false for all possible truth value assignments.
*   **Contingency**: A formula that can be either true or false, depending on the truth values of its variables.
*   **Satisfiable Formula**: A formula for which there exists at least one assignment of truth values that makes the formula true.
*   **Logical Equivalence**: The property of two formulas having identical truth tables.
*   **Literal**: A propositional variable (e.g., $p$) or its negation (e.g., $\neg p$).
*   **Disjunctive Normal Form (DNF)**: A logical formula represented as a disjunction of conjunctive clauses (e.g., $(p \land q) \lor (\neg r \land s)$).
*   **Conjunctive Normal Form (CNF)**: A logical formula represented as a conjunction of disjunctive clauses (e.g., $(p \lor q) \land (\neg r \lor s)$).
*   **Algebraic Normal Form (ANF)**: The representation of a logical function as a polynomial using AND (multiplication) and XOR (addition) operations modulo 2.

---

#### 3. Formulas

*   **Double Negation**: $\neg(\neg p) \equiv p$
*   **De Morgan's Laws**:
    *   $\neg(p \lor q) \equiv \neg p \land \neg q$
    *   $\neg(p \land q) \equiv \neg p \lor \neg q$
*   **Distributive Laws**:
    *   $p \land (q \lor r) \equiv (p \land q) \lor (p \land r)$
    *   $p \lor (q \land r) \equiv (p \lor q) \land (p \lor r)$
*   **Implication**: $p \rightarrow q \equiv \neg p \lor q$
*   **Bi-implication**: $p \leftrightarrow q \equiv (p \land q) \lor (\neg p \land \neg q)$
*   **Algebraic Normal Form (ANF) Conversions**:
    *   $\neg p \equiv p \oplus 1$
    *   $p \lor q \equiv p \oplus q \oplus pq$
    *   $p \land q \equiv pq$
    *   $p \rightarrow q \equiv 1 \oplus p \oplus pq$
    *   $p \leftrightarrow q \equiv 1 \oplus p \oplus q$
*   **ANF Properties (Modulo 2)**:
    *   $p \oplus p \equiv 0$
    *   $p \cdot p \equiv p$

---

#### 4. Mistakes

*   **Incorrectly applying De Morgan's Law**: A common mistake is to distribute the negation without flipping the operator. For example, writing $\neg(a \lor b)$ as $\neg a \lor \neg b$. **Why it's wrong**: De Morgan's Law requires inverting the operator as well, so the correct form is $\neg a \land \neg b$.
*   **Confusing XOR with OR in ANF**: Translating $a \lor b$ as just $a \oplus b$. **Why it's wrong**: Logical OR is not equivalent to XOR. The correct ANF for OR is $a \oplus b \oplus ab$. The term $ab$ corrects for the case where both $a$ and $b$ are true, as $1 \oplus 1 = 0$ but $1 \lor 1 = 1$.
*   **Assuming Distributivity of XOR over AND**: Believing that $x \oplus (y \cdot z) \equiv (x \oplus y) \cdot (x \oplus z)$. **Why it's wrong**: This property does not hold in Boolean algebra. As shown in the slides, a truth table for both sides yields different results. AND distributes over XOR, but not the other way around.
*   **Errors in CNF/DNF Simplification**: Failing to apply the absorption law, $a \lor (a \land b) \equiv a$. A student might leave the expression as is, thinking it's fully simplified. **Why it's wrong**: The absorption law shows that the term $(a \land b)$ is redundant if $a$ is already present in a disjunction, leading to a simpler, equivalent formula.
*   **Forgetting to Negate Inputs for CNF**: When deriving CNF from a truth table, one must create OR clauses for the rows where the output is FALSE. A common error is to use the variables directly instead of their negations. **Why it's wrong**: To make the clause true (and thus not affect the outcome of the AND expression), you must ensure that the specific combination of false inputs evaluates to true in the clause. For a false row like $(a=0, b=1)$, the clause must be $(\neg a \lor b)$ to be a valid part of the CNF. *Correction: The slide says for CNF use $(\neg a \lor b)$ for the row where `a=1,b=0`. This is correct, as for that specific input combination (which makes the original function false), this clause also evaluates to false (`0 v 0 = 0`). The full CNF is a conjunction of such clauses that are `0` only on their specific false line.*

---

#### 5. Examples

##### Example 1: Applying De Morgan's Laws
**Question:** Apply negation and simplify the expression $(\neg a \lor b) \land (c \lor \neg d)$ using De Morgan's Laws.

<details>
<summary>Click to see the solution</summary>

1.  **Apply negation to the entire expression:**
    $$ \neg ((\neg a \lor b) \land (c \lor \neg d)) $$
2.  **Apply De Morgan's Law to the central AND operator.** This flips the AND to an OR and distributes the negation to the two parenthetical clauses.
    $$ \neg(\neg a \lor b) \lor \neg(c \lor \neg d) $$
3.  **Apply De Morgan's Law to each of the two clauses.**
    *   For the first clause: $\neg(\neg a \lor b) \equiv \neg(\neg a) \land \neg b$
    *   For the second clause: $\neg(c \lor \neg d) \equiv \neg c \land \neg(\neg d)$
4.  **Simplify using the Double Negation law** ($\neg(\neg p) \equiv p$).
    *   First clause becomes: $a \land \neg b$
    *   Second clause becomes: $\neg c \land d$
5.  **Combine the simplified clauses with the OR from step 2.**

**Answer:** The simplified expression is **$(a \land \neg b) \lor (\neg c \land d)$**.
</details>

##### Example 2: Finding and Simplifying DNF
**Question:** Find the Disjunctive Normal Form (DNF) for a function $\Phi(x, y, z)$ with the truth table vector $(01111110)$ and simplify it. (The vector represents the function's output for inputs $xyz=000, 001, ..., 111$).

<details>
<summary>Click to see the solution</summary>

1.  **Identify rows where the output is 1.** These correspond to the minterms.
    *   $xyz=001$: $\neg x \land \neg y \land z$
    *   $xyz=010$: $\neg x \land y \land \neg z$
    *   $xyz=011$: $\neg x \land y \land z$
    *   $xyz=100$: $x \land \neg y \land \neg z$
    *   $xyz=101$: $x \land \neg y \land z$
    *   $xyz=110$: $x \land y \land \neg z$
2.  **Write the full DNF by ORing all minterms:**
    $$ (\neg x \land \neg y \land z) \lor (\neg x \land y \land \neg z) \lor (\neg x \land y \land z) \lor (x \land \neg y \land \neg z) \lor (x \land \neg y \land z) \lor (x \land y \land \neg z) $$
3.  **Simplify by grouping terms.**
    *   Group $(\neg x \land y \land \neg z) \lor (\neg x \land y \land z) \rightarrow \neg x \land y$
    *   Group $(\neg x \land \neg y \land z) \lor (\neg x \land y \land z) \rightarrow \neg x \land z$
    *   Group $(x \land \neg y \land z) \lor (\neg x \land \neg y \land z) \rightarrow \neg y \land z$
    *   It is often easier to derive the CNF for the '0' cases and then negate. The function is 0 for $xyz=000$ and $xyz=111$.
4.  **Alternative (easier) Method:** Find CNF of the zeros and apply De Morgan's law.
    *   The function is 0 for $xyz=000$ and $xyz=111$.
    *   The CNF of the function is $(x \lor y \lor z) \land (\neg x \lor \neg y \lor \neg z)$.
    *   The DNF of the *negation* is $(\neg x \land \neg y \land \neg z) \lor (x \land y \land z)$.
    *   Negating this gives back the original function's DNF: $\neg((\neg x \land \neg y \land \neg z) \lor (x \land y \land z)) \equiv (x \lor y \lor z) \land (\neg x \lor \neg y \lor \neg z)$, which is the CNF. Let's return to simplifying the DNF directly.
5.  **Simplify the full DNF using consensus or algebraic manipulation.**
    *   $(\neg x \land \neg y \land z) \lor (\neg x \land y \land z) = \neg x \land z$
    *   $(\neg x \land y \land \neg z) \lor (x \land y \land \neg z) = y \land \neg z$
    *   $(x \land \neg y \land \neg z) \lor (x \land \neg y \land z) = x \land \neg y$
    *   The simplified expression is the OR of these three terms.

**Answer:** The simplified DNF is **$(\neg x \land z) \lor (y \land \neg z) \lor (x \land \neg y)$**.
</details>

##### Example 3: Finding and Simplifying CNF
**Question:** Find the Conjunctive Normal Form (CNF) for a function $\Psi(x, y, z)$ with the truth table vector $(00110000)$ and simplify it.

<details>
<summary>Click to see the solution</summary>

1.  **Identify rows where the output is 0.** These will form the clauses of the CNF.
    *   $xyz=000$: Clause is $(x \lor y \lor z)$
    *   $xyz=001$: Clause is $(x \lor y \lor \neg z)$
    *   $xyz=100$: Clause is $(\neg x \lor y \lor z)$
    *   $xyz=101$: Clause is $(\neg x \lor y \lor \neg z)$
    *   $xyz=110$: Clause is $(\neg x \lor \neg y \lor z)$
    *   $xyz=111$: Clause is $(\neg x \lor \neg y \lor \neg z)$
2.  **Write the full CNF by ANDing all clauses:**
    $$ (x \lor y \lor z) \land (x \lor y \lor \neg z) \land (\neg x \lor y \lor z) \land (\neg x \lor y \lor \neg z) \land (\neg x \lor \neg y \lor z) \land (\neg x \lor \neg y \lor \neg z) $$
3.  **Simplify by grouping terms using the rule $(A \lor B) \land (A \lor \neg B) \equiv A$.**
    *   Group 1 & 2: $(x \lor y \lor z) \land (x \lor y \lor \neg z) \equiv (x \lor y)$
    *   Group 3 & 4: $(\neg x \lor y \lor z) \land (\neg x \lor y \lor \neg z) \equiv (\neg x \lor y)$
    *   Group 5 & 6: $(\neg x \lor \neg y \lor z) \land (\neg x \lor \neg y \lor \neg z) \equiv (\neg x \lor \neg y)$
4.  **Combine the results:**
    $$ (x \lor y) \land (\neg x \lor y) \land (\neg x \lor \neg y) $$
5.  **Simplify further.**
    *   Group the first two simplified clauses: $(x \lor y) \land (\neg x \lor y) \equiv y$.
    *   Now we have: $y \land (\neg x \lor \neg y)$.
6.  **Apply the distributive law:**
    $$ (y \land \neg x) \lor (y \land \neg y) $$
7.  Since $(y \land \neg y) \equiv F$ (contradiction), the expression simplifies to the first term.

**Answer:** The simplified CNF is **$y \land \neg x$**. *(The DNF would be the same)*.
</details>

##### Example 4: Converting to Algebraic Normal Form (ANF)
**Question:** Find the Algebraic Normal Form for the expression $(a \rightarrow \neg b) \land (b \rightarrow a)$.

<details>
<summary>Click to see the solution</summary>

1.  **Translate each part of the expression into its ANF equivalent.**
    *   First, translate the implications:
        *   $a \rightarrow \neg b$: The formula for implication $x \rightarrow y$ is $1 \oplus x \oplus xy$. Here, $x=a$ and $y=\neg b$.
        *   $b \rightarrow a$: Here, $x=b$ and $y=a$. So it becomes $1 \oplus b \oplus ba$.
2.  **Substitute the ANF for negation.** The formula for negation $\neg y$ is $y \oplus 1$.
    *   $\neg b \equiv b \oplus 1$.
3.  **Substitute back into the first implication.**
    *   $a \rightarrow \neg b \equiv 1 \oplus a \oplus a(\neg b) \equiv 1 \oplus a \oplus a(b \oplus 1)$
    *   Distribute $a$: $1 \oplus a \oplus (ab \oplus a)$
    *   Since $a \oplus a = 0$, this simplifies to $1 \oplus ab$.
4.  **The full expression is the AND (multiplication) of the two translated parts.**
    $$ (1 \oplus ab) \cdot (1 \oplus b \oplus ab) $$
5.  **Expand the polynomial (multiply the terms).**
    $$ 1(1 \oplus b \oplus ab) \oplus ab(1 \oplus b \oplus ab) $$
    $$ (1 \oplus b \oplus ab) \oplus (ab \oplus ab^2 \oplus a^2b^2) $$
6.  **Simplify using modulo 2 rules: $x \oplus x = 0$ and $x^2 = x$.**
    *   $ab^2 = ab$ and $a^2b^2 = ab$.
    *   The expression becomes: $1 \oplus b \oplus ab \oplus ab \oplus ab \oplus ab$
7.  **Cancel out pairs.**
    *   $ab \oplus ab = 0$. We have two such pairs.
    *   The expression simplifies to: $1 \oplus b$.

**Answer:** The ANF is **$1 \oplus b$** (which is equivalent to $\neg b$).
</details>